Update F* extraction

libcrux-iot/ml-kem/hax.py
@@ -69,14 +69,16 @@ class extractAction(argparse.Action):
         # Extract ml-kem
         includes = [
             "-**",
-            "+libcrux_iot_ml_kem::spec::*",
-            "+libcrux_iot_ml_kem::vector::portable::arithmetic::**",
-            "+libcrux_iot_ml_kem::vector::portable::ntt::**",
-            "+libcrux_iot_ml_kem::vector::portable::sampling::**",
-            "+libcrux_iot_ml_kem::vector::portable::compress::**",
-            "+libcrux_iot_ml_kem::vector::portable::serialize::**",
+            # "+libcrux_iot_ml_kem::spec::*",
+            "+libcrux_iot_ml_kem::vector::portable::**",
+            # "+libcrux_iot_ml_kem::vector::portable::arithmetic::**",
+            # "+libcrux_iot_ml_kem::vector::portable::ntt::**",
+            # "+libcrux_iot_ml_kem::vector::portable::sampling::**",
+            # "+libcrux_iot_ml_kem::vector::portable::compress::**",
+            # "+libcrux_iot_ml_kem::vector::portable::serialize::**",
         ]
         include_str = " ".join(includes)
+        # interface_include = "+** -libcrux_iot_ml_kem::types -libcrux_iot_ml_kem::constants"
         interface_include = "+** -libcrux_iot_ml_kem::vector::traits -libcrux_iot_ml_kem::types -libcrux_iot_ml_kem::constants"
         cargo_hax_into = [
             "cargo",
