libcrux-iot/ml-kem/proofs/fstar/extraction/Libcrux_iot_ml_kem.Vector.Traits.fst
@@ -12,3 +12,340 @@ let v_INVERSE_OF_MODULUS_MOD_MONTGOMERY_R: u32 = mk_u32 62209
 let v_BARRETT_SHIFT: i32 = mk_i32 26
 
 let v_BARRETT_R: i32 = mk_i32 1 <<! v_BARRETT_SHIFT
+
+class t_Operations (v_Self: Type0) = {
+  [@@@ FStar.Tactics.Typeclasses.no_method]_super_250177790225314374:Core.Marker.t_Copy v_Self;
+  [@@@ FStar.Tactics.Typeclasses.no_method]_super_14156401398203956914:Core.Clone.t_Clone v_Self;
+  f_ZERO_pre:Prims.unit -> Type0;
+  f_ZERO_post:Prims.unit -> v_Self -> Type0;
+  f_ZERO:x0: Prims.unit -> Prims.Pure v_Self (f_ZERO_pre x0) (fun result -> f_ZERO_post x0 result);
+  f_from_i16_array_pre:array: t_Slice i16 -> out: v_Self
+    -> pred: Type0{(Core.Slice.impl__len #i16 array <: usize) =. mk_usize 16 ==> pred};
+  f_from_i16_array_post:t_Slice i16 -> v_Self -> v_Self -> Type0;
+  f_from_i16_array:x0: t_Slice i16 -> x1: v_Self
+    -> Prims.Pure v_Self
+        (f_from_i16_array_pre x0 x1)
+        (fun result -> f_from_i16_array_post x0 x1 result);
+  f_reducing_from_i32_array_pre:array: t_Slice i32 -> out: v_Self
+    -> pred: Type0{(Core.Slice.impl__len #i32 array <: usize) =. mk_usize 16 ==> pred};
+  f_reducing_from_i32_array_post:t_Slice i32 -> v_Self -> v_Self -> Type0;
+  f_reducing_from_i32_array:x0: t_Slice i32 -> x1: v_Self
+    -> Prims.Pure v_Self
+        (f_reducing_from_i32_array_pre x0 x1)
+        (fun result -> f_reducing_from_i32_array_post x0 x1 result);
+  f_to_i16_array_pre:x: v_Self -> out: t_Slice i16
+    -> pred: Type0{(Core.Slice.impl__len #i16 out <: usize) =. mk_usize 16 ==> pred};
+  f_to_i16_array_post:v_Self -> t_Slice i16 -> t_Slice i16 -> Type0;
+  f_to_i16_array:x0: v_Self -> x1: t_Slice i16
+    -> Prims.Pure (t_Slice i16)
+        (f_to_i16_array_pre x0 x1)
+        (fun result -> f_to_i16_array_post x0 x1 result);
+  f_from_bytes_pre:array: t_Slice u8 -> out: v_Self
+    -> pred: Type0{(Core.Slice.impl__len #u8 array <: usize) >=. mk_usize 32 ==> pred};
+  f_from_bytes_post:t_Slice u8 -> v_Self -> v_Self -> Type0;
+  f_from_bytes:x0: t_Slice u8 -> x1: v_Self
+    -> Prims.Pure v_Self (f_from_bytes_pre x0 x1) (fun result -> f_from_bytes_post x0 x1 result);
+  f_to_bytes_pre:x: v_Self -> bytes: t_Slice u8
+    -> pred: Type0{(Core.Slice.impl__len #u8 bytes <: usize) >=. mk_usize 32 ==> pred};
+  f_to_bytes_post:x: v_Self -> bytes: t_Slice u8 -> bytes_future: t_Slice u8
+    -> pred:
+      Type0
+        { pred ==>
+          (Core.Slice.impl__len #u8 bytes_future <: usize) =.
+          (Core.Slice.impl__len #u8 bytes <: usize) };
+  f_to_bytes:x0: v_Self -> x1: t_Slice u8
+    -> Prims.Pure (t_Slice u8) (f_to_bytes_pre x0 x1) (fun result -> f_to_bytes_post x0 x1 result);
+  f_add_pre:v_Self -> v_Self -> Type0;
+  f_add_post:v_Self -> v_Self -> v_Self -> Type0;
+  f_add:x0: v_Self -> x1: v_Self
+    -> Prims.Pure v_Self (f_add_pre x0 x1) (fun result -> f_add_post x0 x1 result);
+  f_sub_pre:v_Self -> v_Self -> Type0;
+  f_sub_post:v_Self -> v_Self -> v_Self -> Type0;
+  f_sub:x0: v_Self -> x1: v_Self
+    -> Prims.Pure v_Self (f_sub_pre x0 x1) (fun result -> f_sub_post x0 x1 result);
+  f_negate_pre:v_Self -> Type0;
+  f_negate_post:v_Self -> v_Self -> Type0;
+  f_negate:x0: v_Self -> Prims.Pure v_Self (f_negate_pre x0) (fun result -> f_negate_post x0 result);
+  f_multiply_by_constant_pre:v_Self -> i16 -> Type0;
+  f_multiply_by_constant_post:v_Self -> i16 -> v_Self -> Type0;
+  f_multiply_by_constant:x0: v_Self -> x1: i16
+    -> Prims.Pure v_Self
+        (f_multiply_by_constant_pre x0 x1)
+        (fun result -> f_multiply_by_constant_post x0 x1 result);
+  f_bitwise_and_with_constant_pre:v_Self -> i16 -> Type0;
+  f_bitwise_and_with_constant_post:v_Self -> i16 -> v_Self -> Type0;
+  f_bitwise_and_with_constant:x0: v_Self -> x1: i16
+    -> Prims.Pure v_Self
+        (f_bitwise_and_with_constant_pre x0 x1)
+        (fun result -> f_bitwise_and_with_constant_post x0 x1 result);
+  f_shift_right_pre:v_SHIFT_BY: i32 -> vec: v_Self
+    -> pred: Type0{v_SHIFT_BY >=. mk_i32 0 && v_SHIFT_BY <. mk_i32 16 ==> pred};
+  f_shift_right_post:v_SHIFT_BY: i32 -> v_Self -> v_Self -> Type0;
+  f_shift_right:v_SHIFT_BY: i32 -> x0: v_Self
+    -> Prims.Pure v_Self
+        (f_shift_right_pre v_SHIFT_BY x0)
+        (fun result -> f_shift_right_post v_SHIFT_BY x0 result);
+  f_cond_subtract_3329__pre:v_Self -> Type0;
+  f_cond_subtract_3329__post:v_Self -> v_Self -> Type0;
+  f_cond_subtract_3329_:x0: v_Self
+    -> Prims.Pure v_Self
+        (f_cond_subtract_3329__pre x0)
+        (fun result -> f_cond_subtract_3329__post x0 result);
+  f_barrett_reduce_pre:v_Self -> Type0;
+  f_barrett_reduce_post:v_Self -> v_Self -> Type0;
+  f_barrett_reduce:x0: v_Self
+    -> Prims.Pure v_Self (f_barrett_reduce_pre x0) (fun result -> f_barrett_reduce_post x0 result);
+  f_montgomery_multiply_by_constant_pre:v_Self -> i16 -> Type0;
+  f_montgomery_multiply_by_constant_post:v_Self -> i16 -> v_Self -> Type0;
+  f_montgomery_multiply_by_constant:x0: v_Self -> x1: i16
+    -> Prims.Pure v_Self
+        (f_montgomery_multiply_by_constant_pre x0 x1)
+        (fun result -> f_montgomery_multiply_by_constant_post x0 x1 result);
+  f_compress_1__pre:v_Self -> Type0;
+  f_compress_1__post:v_Self -> v_Self -> Type0;
+  f_compress_1_:x0: v_Self
+    -> Prims.Pure v_Self (f_compress_1__pre x0) (fun result -> f_compress_1__post x0 result);
+  f_compress_pre:v_COEFFICIENT_BITS: i32 -> vec: v_Self
+    -> pred: Type0{v_COEFFICIENT_BITS >=. mk_i32 0 && v_COEFFICIENT_BITS <=. mk_i32 16 ==> pred};
+  f_compress_post:v_COEFFICIENT_BITS: i32 -> v_Self -> v_Self -> Type0;
+  f_compress:v_COEFFICIENT_BITS: i32 -> x0: v_Self
+    -> Prims.Pure v_Self
+        (f_compress_pre v_COEFFICIENT_BITS x0)
+        (fun result -> f_compress_post v_COEFFICIENT_BITS x0 result);
+  f_decompress_ciphertext_coefficient_pre:v_COEFFICIENT_BITS: i32 -> vec: v_Self
+    -> pred: Type0{mk_i32 0 <=. v_COEFFICIENT_BITS && v_COEFFICIENT_BITS <. mk_i32 31 ==> pred};
+  f_decompress_ciphertext_coefficient_post:v_COEFFICIENT_BITS: i32 -> v_Self -> v_Self -> Type0;
+  f_decompress_ciphertext_coefficient:v_COEFFICIENT_BITS: i32 -> x0: v_Self
+    -> Prims.Pure v_Self
+        (f_decompress_ciphertext_coefficient_pre v_COEFFICIENT_BITS x0)
+        (fun result -> f_decompress_ciphertext_coefficient_post v_COEFFICIENT_BITS x0 result);
+  f_ntt_layer_1_step_pre:v_Self -> i16 -> i16 -> i16 -> i16 -> Type0;
+  f_ntt_layer_1_step_post:v_Self -> i16 -> i16 -> i16 -> i16 -> v_Self -> Type0;
+  f_ntt_layer_1_step:x0: v_Self -> x1: i16 -> x2: i16 -> x3: i16 -> x4: i16
+    -> Prims.Pure v_Self
+        (f_ntt_layer_1_step_pre x0 x1 x2 x3 x4)
+        (fun result -> f_ntt_layer_1_step_post x0 x1 x2 x3 x4 result);
+  f_ntt_layer_2_step_pre:v_Self -> i16 -> i16 -> Type0;
+  f_ntt_layer_2_step_post:v_Self -> i16 -> i16 -> v_Self -> Type0;
+  f_ntt_layer_2_step:x0: v_Self -> x1: i16 -> x2: i16
+    -> Prims.Pure v_Self
+        (f_ntt_layer_2_step_pre x0 x1 x2)
+        (fun result -> f_ntt_layer_2_step_post x0 x1 x2 result);
+  f_ntt_layer_3_step_pre:v_Self -> i16 -> Type0;
+  f_ntt_layer_3_step_post:v_Self -> i16 -> v_Self -> Type0;
+  f_ntt_layer_3_step:x0: v_Self -> x1: i16
+    -> Prims.Pure v_Self
+        (f_ntt_layer_3_step_pre x0 x1)
+        (fun result -> f_ntt_layer_3_step_post x0 x1 result);
+  f_inv_ntt_layer_1_step_pre:v_Self -> i16 -> i16 -> i16 -> i16 -> Type0;
+  f_inv_ntt_layer_1_step_post:v_Self -> i16 -> i16 -> i16 -> i16 -> v_Self -> Type0;
+  f_inv_ntt_layer_1_step:x0: v_Self -> x1: i16 -> x2: i16 -> x3: i16 -> x4: i16
+    -> Prims.Pure v_Self
+        (f_inv_ntt_layer_1_step_pre x0 x1 x2 x3 x4)
+        (fun result -> f_inv_ntt_layer_1_step_post x0 x1 x2 x3 x4 result);
+  f_inv_ntt_layer_2_step_pre:v_Self -> i16 -> i16 -> Type0;
+  f_inv_ntt_layer_2_step_post:v_Self -> i16 -> i16 -> v_Self -> Type0;
+  f_inv_ntt_layer_2_step:x0: v_Self -> x1: i16 -> x2: i16
+    -> Prims.Pure v_Self
+        (f_inv_ntt_layer_2_step_pre x0 x1 x2)
+        (fun result -> f_inv_ntt_layer_2_step_post x0 x1 x2 result);
+  f_inv_ntt_layer_3_step_pre:v_Self -> i16 -> Type0;
+  f_inv_ntt_layer_3_step_post:v_Self -> i16 -> v_Self -> Type0;
+  f_inv_ntt_layer_3_step:x0: v_Self -> x1: i16
+    -> Prims.Pure v_Self
+        (f_inv_ntt_layer_3_step_pre x0 x1)
+        (fun result -> f_inv_ntt_layer_3_step_post x0 x1 result);
+  f_accumulating_ntt_multiply_pre:
+      lhs: v_Self ->
+      rhs: v_Self ->
+      out: t_Slice i32 ->
+      zeta0: i16 ->
+      zeta1: i16 ->
+      zeta2: i16 ->
+      zeta3: i16
+    -> pred: Type0{(Core.Slice.impl__len #i32 out <: usize) >=. mk_usize 16 ==> pred};
+  f_accumulating_ntt_multiply_post:
+      v_Self ->
+      v_Self ->
+      t_Slice i32 ->
+      i16 ->
+      i16 ->
+      i16 ->
+      i16 ->
+      t_Slice i32
+    -> Type0;
+  f_accumulating_ntt_multiply:
+      x0: v_Self ->
+      x1: v_Self ->
+      x2: t_Slice i32 ->
+      x3: i16 ->
+      x4: i16 ->
+      x5: i16 ->
+      x6: i16
+    -> Prims.Pure (t_Slice i32)
+        (f_accumulating_ntt_multiply_pre x0 x1 x2 x3 x4 x5 x6)
+        (fun result -> f_accumulating_ntt_multiply_post x0 x1 x2 x3 x4 x5 x6 result);
+  f_accumulating_ntt_multiply_fill_cache_pre:
+      lhs: v_Self ->
+      rhs: v_Self ->
+      out: t_Slice i32 ->
+      cache: v_Self ->
+      zeta0: i16 ->
+      zeta1: i16 ->
+      zeta2: i16 ->
+      zeta3: i16
+    -> pred: Type0{(Core.Slice.impl__len #i32 out <: usize) >=. mk_usize 16 ==> pred};
+  f_accumulating_ntt_multiply_fill_cache_post:
+      v_Self ->
+      v_Self ->
+      t_Slice i32 ->
+      v_Self ->
+      i16 ->
+      i16 ->
+      i16 ->
+      i16 ->
+      (t_Slice i32 & v_Self)
+    -> Type0;
+  f_accumulating_ntt_multiply_fill_cache:
+      x0: v_Self ->
+      x1: v_Self ->
+      x2: t_Slice i32 ->
+      x3: v_Self ->
+      x4: i16 ->
+      x5: i16 ->
+      x6: i16 ->
+      x7: i16
+    -> Prims.Pure (t_Slice i32 & v_Self)
+        (f_accumulating_ntt_multiply_fill_cache_pre x0 x1 x2 x3 x4 x5 x6 x7)
+        (fun result -> f_accumulating_ntt_multiply_fill_cache_post x0 x1 x2 x3 x4 x5 x6 x7 result);
+  f_accumulating_ntt_multiply_use_cache_pre:
+      lhs: v_Self ->
+      rhs: v_Self ->
+      out: t_Slice i32 ->
+      cache: v_Self
+    -> pred: Type0{(Core.Slice.impl__len #i32 out <: usize) >=. mk_usize 16 ==> pred};
+  f_accumulating_ntt_multiply_use_cache_post:
+      v_Self ->
+      v_Self ->
+      t_Slice i32 ->
+      v_Self ->
+      t_Slice i32
+    -> Type0;
+  f_accumulating_ntt_multiply_use_cache:x0: v_Self -> x1: v_Self -> x2: t_Slice i32 -> x3: v_Self
+    -> Prims.Pure (t_Slice i32)
+        (f_accumulating_ntt_multiply_use_cache_pre x0 x1 x2 x3)
+        (fun result -> f_accumulating_ntt_multiply_use_cache_post x0 x1 x2 x3 result);
+  f_serialize_1__pre:a: v_Self -> out: t_Slice u8
+    -> pred: Type0{(Core.Slice.impl__len #u8 out <: usize) =. mk_usize 2 ==> pred};
+  f_serialize_1__post:a: v_Self -> out: t_Slice u8 -> out_future: t_Slice u8
+    -> pred: Type0{pred ==> (Core.Slice.impl__len #u8 out_future <: usize) =. mk_usize 2};
+  f_serialize_1_:x0: v_Self -> x1: t_Slice u8
+    -> Prims.Pure (t_Slice u8)
+        (f_serialize_1__pre x0 x1)
+        (fun result -> f_serialize_1__post x0 x1 result);
+  f_deserialize_1__pre:a: t_Slice u8 -> out: v_Self
+    -> pred: Type0{(Core.Slice.impl__len #u8 a <: usize) =. mk_usize 2 ==> pred};
+  f_deserialize_1__post:t_Slice u8 -> v_Self -> v_Self -> Type0;
+  f_deserialize_1_:x0: t_Slice u8 -> x1: v_Self
+    -> Prims.Pure v_Self
+        (f_deserialize_1__pre x0 x1)
+        (fun result -> f_deserialize_1__post x0 x1 result);
+  f_serialize_4__pre:a: v_Self -> out: t_Slice u8
+    -> pred: Type0{(Core.Slice.impl__len #u8 out <: usize) =. mk_usize 8 ==> pred};
+  f_serialize_4__post:a: v_Self -> out: t_Slice u8 -> out_future: t_Slice u8
+    -> pred: Type0{pred ==> (Core.Slice.impl__len #u8 out_future <: usize) =. mk_usize 8};
+  f_serialize_4_:x0: v_Self -> x1: t_Slice u8
+    -> Prims.Pure (t_Slice u8)
+        (f_serialize_4__pre x0 x1)
+        (fun result -> f_serialize_4__post x0 x1 result);
+  f_deserialize_4__pre:a: t_Slice u8 -> out: v_Self
+    -> pred: Type0{(Core.Slice.impl__len #u8 a <: usize) =. mk_usize 8 ==> pred};
+  f_deserialize_4__post:t_Slice u8 -> v_Self -> v_Self -> Type0;
+  f_deserialize_4_:x0: t_Slice u8 -> x1: v_Self
+    -> Prims.Pure v_Self
+        (f_deserialize_4__pre x0 x1)
+        (fun result -> f_deserialize_4__post x0 x1 result);
+  f_serialize_5__pre:a: v_Self -> out: t_Slice u8
+    -> pred: Type0{(Core.Slice.impl__len #u8 out <: usize) =. mk_usize 10 ==> pred};
+  f_serialize_5__post:a: v_Self -> out: t_Slice u8 -> out_future: t_Slice u8
+    -> pred: Type0{pred ==> (Core.Slice.impl__len #u8 out_future <: usize) =. mk_usize 10};
+  f_serialize_5_:x0: v_Self -> x1: t_Slice u8
+    -> Prims.Pure (t_Slice u8)
+        (f_serialize_5__pre x0 x1)
+        (fun result -> f_serialize_5__post x0 x1 result);
+  f_deserialize_5__pre:a: t_Slice u8 -> out: v_Self
+    -> pred: Type0{(Core.Slice.impl__len #u8 a <: usize) =. mk_usize 10 ==> pred};
+  f_deserialize_5__post:t_Slice u8 -> v_Self -> v_Self -> Type0;
+  f_deserialize_5_:x0: t_Slice u8 -> x1: v_Self
+    -> Prims.Pure v_Self
+        (f_deserialize_5__pre x0 x1)
+        (fun result -> f_deserialize_5__post x0 x1 result);
+  f_serialize_10__pre:a: v_Self -> out: t_Slice u8
+    -> pred: Type0{(Core.Slice.impl__len #u8 out <: usize) =. mk_usize 20 ==> pred};
+  f_serialize_10__post:a: v_Self -> out: t_Slice u8 -> out_future: t_Slice u8
+    -> pred: Type0{pred ==> (Core.Slice.impl__len #u8 out_future <: usize) =. mk_usize 20};
+  f_serialize_10_:x0: v_Self -> x1: t_Slice u8
+    -> Prims.Pure (t_Slice u8)
+        (f_serialize_10__pre x0 x1)
+        (fun result -> f_serialize_10__post x0 x1 result);
+  f_deserialize_10__pre:a: t_Slice u8 -> out: v_Self
+    -> pred: Type0{(Core.Slice.impl__len #u8 a <: usize) =. mk_usize 20 ==> pred};
+  f_deserialize_10__post:t_Slice u8 -> v_Self -> v_Self -> Type0;
+  f_deserialize_10_:x0: t_Slice u8 -> x1: v_Self
+    -> Prims.Pure v_Self
+        (f_deserialize_10__pre x0 x1)
+        (fun result -> f_deserialize_10__post x0 x1 result);
+  f_serialize_11__pre:a: v_Self -> out: t_Slice u8
+    -> pred: Type0{(Core.Slice.impl__len #u8 out <: usize) =. mk_usize 22 ==> pred};
+  f_serialize_11__post:a: v_Self -> out: t_Slice u8 -> out_future: t_Slice u8
+    -> pred: Type0{pred ==> (Core.Slice.impl__len #u8 out_future <: usize) =. mk_usize 22};
+  f_serialize_11_:x0: v_Self -> x1: t_Slice u8
+    -> Prims.Pure (t_Slice u8)
+        (f_serialize_11__pre x0 x1)
+        (fun result -> f_serialize_11__post x0 x1 result);
+  f_deserialize_11__pre:a: t_Slice u8 -> out: v_Self
+    -> pred: Type0{(Core.Slice.impl__len #u8 a <: usize) =. mk_usize 22 ==> pred};
+  f_deserialize_11__post:t_Slice u8 -> v_Self -> v_Self -> Type0;
+  f_deserialize_11_:x0: t_Slice u8 -> x1: v_Self
+    -> Prims.Pure v_Self
+        (f_deserialize_11__pre x0 x1)
+        (fun result -> f_deserialize_11__post x0 x1 result);
+  f_serialize_12__pre:a: v_Self -> out: t_Slice u8
+    -> pred: Type0{(Core.Slice.impl__len #u8 out <: usize) =. mk_usize 24 ==> pred};
+  f_serialize_12__post:a: v_Self -> out: t_Slice u8 -> out_future: t_Slice u8
+    -> pred: Type0{pred ==> (Core.Slice.impl__len #u8 out_future <: usize) =. mk_usize 24};
+  f_serialize_12_:x0: v_Self -> x1: t_Slice u8
+    -> Prims.Pure (t_Slice u8)
+        (f_serialize_12__pre x0 x1)
+        (fun result -> f_serialize_12__post x0 x1 result);
+  f_deserialize_12__pre:a: t_Slice u8 -> out: v_Self
+    -> pred: Type0{(Core.Slice.impl__len #u8 a <: usize) =. mk_usize 24 ==> pred};
+  f_deserialize_12__post:t_Slice u8 -> v_Self -> v_Self -> Type0;
+  f_deserialize_12_:x0: t_Slice u8 -> x1: v_Self
+    -> Prims.Pure v_Self
+        (f_deserialize_12__pre x0 x1)
+        (fun result -> f_deserialize_12__post x0 x1 result);
+  f_rej_sample_pre:a: t_Slice u8 -> out: t_Slice i16
+    -> pred:
+      Type0
+        { (Core.Slice.impl__len #u8 a <: usize) =. mk_usize 24 &&
+          (Core.Slice.impl__len #i16 out <: usize) =. mk_usize 16 ==>
+          pred };
+  f_rej_sample_post:a: t_Slice u8 -> out: t_Slice i16 -> x: (t_Slice i16 & usize)
+    -> pred:
+      Type0
+        { pred ==>
+          (let out_future, result:(t_Slice i16 & usize) = x in
+            result <=. mk_usize 16 && (Core.Slice.impl__len #i16 out_future <: usize) =. mk_usize 16
+          ) };
+  f_rej_sample:x0: t_Slice u8 -> x1: t_Slice i16
+    -> Prims.Pure (t_Slice i16 & usize)
+        (f_rej_sample_pre x0 x1)
+        (fun result -> f_rej_sample_post x0 x1 result)
+}
+
+[@@ FStar.Tactics.Typeclasses.tcinstance]
+let _ = fun (v_Self:Type0) {|i: t_Operations v_Self|} -> i._super_250177790225314374
+
+[@@ FStar.Tactics.Typeclasses.tcinstance]
+let _ = fun (v_Self:Type0) {|i: t_Operations v_Self|} -> i._super_14156401398203956914
