libcrux-iot/ml-kem/proofs/fstar/extraction/Libcrux_iot_ml_kem.Vector.Portable.fsti
@@ -1,0 +1,17 @@
+module Libcrux_iot_ml_kem.Vector.Portable
+#set-options "--fuel 0 --ifuel 1 --z3rlimit 80"
+open Core
+open FStar.Mul
+
+let _ =
+  (* This module has implicit dependencies, here we make them explicit. *)
+  (* The implicit dependencies arise from typeclasses instances. *)
+  let open Libcrux_iot_ml_kem.Vector.Portable.Vector_type in
+  let open Libcrux_secrets.Int.Classify_public in
+  let open Libcrux_secrets.Int.Public_integers in
+  let open Libcrux_secrets.Traits in
+  ()
+
+[@@ FStar.Tactics.Typeclasses.tcinstance]
+val impl:Libcrux_iot_ml_kem.Vector.Traits.t_Operations
+Libcrux_iot_ml_kem.Vector.Portable.Vector_type.t_PortableVector
