libcrux-iot/ml-kem/proofs/fstar/extraction/Libcrux_iot_ml_kem.Vector.Traits.Spec.fst
@@ -1,0 +1,95 @@
+module Libcrux_iot_ml_kem.Vector.Traits.Spec
+#set-options "--fuel 0 --ifuel 1 --z3rlimit 80"
+open Core
+open FStar.Mul
+
+let add_pre (lhs rhs: t_Array i16 (mk_usize 16)) : Hax_lib.Prop.t_Prop =
+  forall i. i < 16 ==> Spec.Utils.is_intb (pow2 15 - 1) (v (Seq.index lhs i) + v (Seq.index rhs i))
+
+let add_post (lhs rhs result: t_Array i16 (mk_usize 16)) : Hax_lib.Prop.t_Prop =
+  forall i. i < 16 ==> (v (Seq.index result i) == v (Seq.index lhs i) + v (Seq.index rhs i))
+
+let sub_pre (lhs rhs: t_Array i16 (mk_usize 16)) : Hax_lib.Prop.t_Prop =
+  forall i. i < 16 ==> Spec.Utils.is_intb (pow2 15 - 1) (v (Seq.index lhs i) - v (Seq.index rhs i))
+
+let sub_post (lhs rhs result: t_Array i16 (mk_usize 16)) : Hax_lib.Prop.t_Prop =
+  forall i. i < 16 ==> (v (Seq.index result i) == v (Seq.index lhs i) - v (Seq.index rhs i))
+
+let negate_pre (vec: t_Array i16 (mk_usize 16)) : Hax_lib.Prop.t_Prop =
+  forall i. i < 16 ==> Spec.Utils.is_intb (pow2 15 - 1) (v (Seq.index vec i))
+
+let negate_post (vec result: t_Array i16 (mk_usize 16)) : Hax_lib.Prop.t_Prop =
+  forall i. i < 16 ==> v (Seq.index result i) == - (v (Seq.index vec i))
+
+let multiply_by_constant_pre (vec: t_Array i16 (mk_usize 16)) (c: i16) : Hax_lib.Prop.t_Prop =
+  forall i. i < 16 ==> Spec.Utils.is_intb (pow2 15 - 1) (v (Seq.index vec i) * v c)
+
+let multiply_by_constant_post
+      (vec: t_Array i16 (mk_usize 16))
+      (c: i16)
+      (result: t_Array i16 (mk_usize 16))
+    : Hax_lib.Prop.t_Prop = forall i. v (Seq.index result i) == v (Seq.index vec i) * v c
+
+let bitwise_and_with_constant_constant_post
+      (vec: t_Array i16 (mk_usize 16))
+      (c: i16)
+      (result: t_Array i16 (mk_usize 16))
+    : Hax_lib.Prop.t_Prop = result == Spec.Utils.map_array (fun x -> x &. c) vec
+
+let shift_right_post
+      (vec: t_Array i16 (mk_usize 16))
+      (shift_by: i32)
+      (result: t_Array i16 (mk_usize 16))
+    : Hax_lib.Prop.t_Prop =
+  (v shift_by >= 0 /\ v shift_by < 16) ==>
+  result == Spec.Utils.map_array (fun x -> x >>! shift_by) vec
+
+let cond_subtract_3329_pre (vec: t_Array i16 (mk_usize 16)) : Hax_lib.Prop.t_Prop =
+  Spec.Utils.is_i16b_array (pow2 12 - 1) vec
+
+let cond_subtract_3329_post (vec result: t_Array i16 (mk_usize 16)) : Hax_lib.Prop.t_Prop =
+  result ==
+  Spec.Utils.map_array (fun x -> if x >=. (mk_i16 3329) then x -! (mk_i16 3329) else x) vec
+
+let barrett_reduce_pre (vec: t_Array i16 (mk_usize 16)) : Hax_lib.Prop.t_Prop =
+  Spec.Utils.is_i16b_array 28296 vec
+
+let barrett_reduce_post (vec result: t_Array i16 (mk_usize 16)) : Hax_lib.Prop.t_Prop =
+  Spec.Utils.is_i16b_array 3328 result /\
+  (forall i. (v (Seq.index result i) % 3329) == (v (Seq.index vec i) % 3329))
+
+let montgomery_multiply_by_constant_pre (vec: t_Array i16 (mk_usize 16)) (c: i16)
+    : Hax_lib.Prop.t_Prop = Spec.Utils.is_i16b 1664 c
+
+let montgomery_multiply_by_constant_post
+      (vec: t_Array i16 (mk_usize 16))
+      (c: i16)
+      (result: t_Array i16 (mk_usize 16))
+    : Hax_lib.Prop.t_Prop =
+  Spec.Utils.is_i16b_array 3328 result /\
+  (forall i. ((v (Seq.index result i) % 3329) == (v (Seq.index vec i) * v c * 169) % 3329))
+
+let compress_1_pre (vec: t_Array i16 (mk_usize 16)) : Hax_lib.Prop.t_Prop =
+  forall i. v (Seq.index vec i) >= 0 /\ v (Seq.index vec i) < 3329
+
+let compress_1_post (vec result: t_Array i16 (mk_usize 16)) : Hax_lib.Prop.t_Prop =
+  forall i. bounded (Seq.index result i) 1
+
+let compress_pre (vec: t_Array i16 (mk_usize 16)) (coefficient_bits: i32) : Hax_lib.Prop.t_Prop =
+  (v coefficient_bits == 4 \/ v coefficient_bits == 5 \/ v coefficient_bits == 10 \/
+    v coefficient_bits == 11) /\ (forall i. v (Seq.index vec i) >= 0 /\ v (Seq.index vec i) < 3329)
+
+let compress_post
+      (vec: t_Array i16 (mk_usize 16))
+      (coefficient_bits: i32)
+      (result: t_Array i16 (mk_usize 16))
+    : Hax_lib.Prop.t_Prop =
+  (v coefficient_bits == 4 \/ v coefficient_bits == 5 \/ v coefficient_bits == 10 \/
+    v coefficient_bits == 11) ==>
+  (forall i. bounded (Seq.index result i) (v coefficient_bits))
+
+let decompress_ciphertext_coefficient_pre (vec: t_Array i16 (mk_usize 16)) (coefficient_bits: i32)
+    : Hax_lib.Prop.t_Prop =
+  (v coefficient_bits == 4 \/ v coefficient_bits == 5 \/ v coefficient_bits == 10 \/
+    v coefficient_bits == 11) /\
+  (forall i. v (Seq.index vec i) >= 0 /\ v (Seq.index vec i) < pow2 (v coefficient_bits))
